\section{Representations}

\subsection{Induced Representations}
We assume $G$ is discrete group.
Let $H < G$ be a subgroup of $G$.
In the case of locally compact groups, if $H$ is open or compact open, probably OK.
Let $\sigma$ be a unitary representation of $H$.
Let $q:G \rightarrow G/H$ be a quotient map.
\begin{align*}
  \mathcal{F}_0 := \{f \in C_c(G,H_\sigma) | q(supp(f)):compact,\, f(y \xi) = \sigma(\xi^{-1})f(y) \; (y \in G,\; \xi \in H)\}.
\end{align*}
For $f$, $g \in \mathcal{F}_0$,
\begin{align*}
  \<f,g\> := \int_{G/H}\<f(x),g(x)\>_\sigma d \mu(xH).
\end{align*}

We define $\mathcal{F}$ by the completion of $\mathcal{F}_0$ w.r.t. this inner product.
$G$ acts on $\mathcal{F}$ by left transformation, denoted by $\ind_H^G(\sigma)$
\begin{remark}
  If $\sigma$ is a trivial representation, $\ind_H^G(\sigma)$ is the natural representation of $G$ on $l^2(G/H)$ by left transformation.
\end{remark}
\begin{proposition}
  $\ind_H^G(\lambda_H) \cong \lambda_G$.
\end{proposition}

\begin{proof}
  \begin{align*}
    \mathcal{F} := \{f \in l^2(G,l^2(H_\sigma)) | ||f|| < \infty (not \; l^2) ,\; f(y\xi)(s) = f(y)(\xi s) \;(y \in G, \xi,s \in H)\}.
  \end{align*}
  We define $\Phi : l^2(G) \rightarrow \mathcal{F}$ by $\Phi(f)(y)(\xi) := f(y\xi)$ for $f \in l^2(G)$, $y \in G$, $\xi \in H)$.
  linear is OK.

  Surjectivity: For $f \in \mathcal{F}$, $g(y):= f(y,e)$.

  Inner product preserving: For $f, g \in l^2(G)$,
  \begin{align*}
    \<\Phi(f),\Phi(g)\> &= \int_{G/H} \<\Phi(f)(x),\Phi(g)(x)\>_\sigma d \mu_{G/H}(xH)\\
    &=\int_{G/H} \int_H \Phi(f)(x,s) \overline{\Phi(g)(x,s)} d\mu_H(s)d\mu_{G/H}(xH)\\
    &=\int_{G/H} \int_H f(xs) \overline{g(xs)} d\mu_H(s)d\mu_{G/H}(xH)\\
    &=\int_Gf(x)\overline{g(x)}d\mu_G(x) = \<f,g\>
  \end{align*}
  We suffices to check the following diagram is commutative.
  \[
  \xymatrix{
    l^2(G) \ar[r]^{\lambda_G} \ar[d]^{\Phi}& l^2(G) \ar[d]^{\Phi} \\
    \mathcal{F} \ar[r]^{\ind_H^G(\lambda_H)} & \mathcal{F}.
  }
  \]
  Let $\sigma = \ind_H^G(\lambda_H)$.
  For $f \in l^2(G)$, $g, y \in G$, $\xi \in H$,
  \begin{align*}
    (\sigma(g) \circ \Phi)(f)(y, \xi) &= \sigma(g)( \Phi(f)) (y,\xi) = \Phi(f)(g^{-1}y,\xi) = f(g^{-1}y\xi),\\
    (\Phi \circ \lambda_G(g))(f)(y,\xi) &= \Phi(\lambda_G(g)(f))(y,\xi) = (\lambda_G(g)(f))(y\xi) = f(g^{-1}y\xi).
  \end{align*}
\end{proof}
